<section xml:id="constrained-optimization">
  <title>Constrained Optimization</title>
  <p>
    Let's reconsider the box-in-a-sphere problem of <xref ref="example-box-sphere">Example</xref>.
    Instead of working inside the sphere,
    we could just consider a prism centred at the origin with positive octant vertex <m>(a,b,c)</m> and volume <m>8abc</m>.
    That maximized by itself will diverge to <m>\infty</m>,
    since we have nothing to bound the prism.
    However, we can consider the <em>constraint</em>
    <m>x^2 + y^2 + z^2 = r^2</m> for some fixed <m>r</m>.
  </p>
  <p>
    The idea, in general, is to ask when a function
    <m>f(x_1, x_2, \ldots,
    x_n)</m> is optimized subject to one
    (or more)
    constraints <m>g(x_1, x_2, \ldots x_n) = c</m>.
    Let's first think of this geometrically.
    If both <m>f</m> and <m>g</m> were functions of two variables,
    we could draw contour plots.
    <m>g(x,y) = c</m> would be a fixed countour line for <m>g</m>,
    and we would be asking for maximum of <m>f</m> along that contour line.
    We can notice that such a maximum occurs where a countour line for <m>f</m> touches the contour line <m>g(x,y) = c</m> and then backs off.
    That is, the maximum occurs where the contour lines are tangent.
  </p>
  <p>
    But the contour lines are level sets,
    which are defined by their normals.
    The normals are given by gradients.
    If the level sets are tangent to each other,
    that means the gradients must be in the same direction
    (up to a sign).
    That is, this optimization occurs when <m>\nabla f \parallel \nabla g</m>.
    We can express this as <m>\nabla f = \lambda \nabla g</m> for some real constant <m>\lambda \neq 0</m>.
  </p>
  <p>
    This holds in any dinemsion:
    the level sets will be tangent and there will be a constant <m>\lambda</m> with <m>\nabla f = \lambda \nabla g</m>.
    To optimize with constraint,
    we now have a system of equation in <m>n+1</m> variables,
    the <m>x_i</m> and <m>\lambda</m>:
    <m>\nabla f = \lambda \nabla g</m> and <m>g(x_1, x_2, \ldots,
    v_n) = c</m>.
    To optimize the situation, we try to solve this system.
    This method is called the method of Lagrange Multipliers.
  </p>
  <p>
    (Historically,
    the connection to the mathematician Lagrange comes from a <em>Lagrangian</em>
    of the form <m>f + \lambda g</m>.
    We're essentially looking for critical points of this Lagrangian).
  </p>
  <example>
    <statement>
      <p>
        What is the largest rectangle with fixed perimeter <m>p</m>?
        The rectangle has length <m>l</m> and height <m>h</m>,
        with area <m>A(h,l) = hl</m>.
        The constraint is the fixed perimeter <m>2h + 2l = p</m>,
        so the function is <m>g(h,l) = 2h + 2l</m>.
        The gradients are <m>\nabla A = (l,h)</m> and <m>\nabla g = (2,2)</m>.
        The equation <m>\nabla A = \lambda \nabla g</m> is two equations:
        <m>h = 2\lambda</m> and <m>l = 2 \lambda</m>.
        We can substitute these into the constrait
        <m>2h + 2l = p</m> to get <m>8 \lambda = p</m> so
        <m>\lambda = p/8</m> and <m>h = l = 2 \lambda = p/4</m>.
        The area is then <m>p^2/16</m>.
      </p>
    </statement>
  </example>
  <example>
    <statement>
      <p>
        Let's actually do the motivating <xref ref="example-box-sphere">Example</xref> with Lagrange Multipliers.
        <men>
          \begin{array}{*4{>{\displaystyle}l}} V(x,y,z) = 8xyz \amp  \amp \hspace{1cm} g(x,y,z) = x^2 + y^2 + z^2 = r^2 \amp  \\[1em] \nabla V = (8yx,8xz,8xy) \amp  \amp \hspace{1cm} \nabla g = (2x, 2y, 2z) \amp  \\[1em] \nabla V = \lambda \nabla g \amp  \amp  \amp  \\[1em] 8yz = \lambda 2x \amp \hspace{1cm} 8xz = \lambda 2y \amp \hspace{2cm} 8xy = \lambda 2z \amp \end{array}
        </men>
      </p>
      <p>
        We will use the first of the three equations to isolate for <m>x</m>,
        which we substitute in the second.
        <md>
          <mrow>x \amp  = \frac{1}{\lambda} 4yz \hspace{1cm} \frac{8}{\lambda} 4yz^2 = \lambda 2y</mrow>
          <intertext>We solve for <m>z</m> (cancelling <m>y</m>, so careful with the possibility of <m>y=0</m>.)</intertext>
          <mrow>16z^2 \amp  = \lambda^2 \implies z = \frac{\lambda}{4}</mrow>
          <mrow>\frac{8}{\lambda} 4 y^2 z \amp  = \lambda 2z</mrow>
          <intertext>Since everything in this question is symmetric, we apply the same reasoning with different variables.</intertext>
          <mrow>y \amp  = \frac{\lambda}{4} \hspace{2cm} x = \frac{\lambda}{4}</mrow>
          <intertext>We put <m>x</m>, <m>y</m> and <m>z</m> into the constraint to solve for <m>\lambda</m>.</intertext>
          <mrow>x^2 + y^2 + z^2 \amp  = \frac{3\lambda^2}{16} = r^2 \implies \lambda = \frac{4r}{\sqrt{3}}</mrow>
          <intertext>Then we use the value of <m>\gamma</m> to give the values of the variables.</intertext>
          <mrow>x = y = z \amp  = \frac{r}{\sqrt{3}}</mrow>
          <mrow>V \amp  = \frac{8r^3}{3\sqrt{3}}</mrow>
        </md>
      </p>
      <p>
        We recovered the same maximal area as before.
        We don't have to worry about the <m>y=0</m> possibility that we noted (or likewise <m>x=0</m> and <m>z=0)</m>,
        since any solution in that case would lead to zero volume,
        which is certainly not maximal.
      </p>
    </statement>
  </example>
  <example>
    <statement>
      <p>
        Instead of a sphere,
        we could ask for the largest box inside an ellipsoid with equation <m>\frac{x^2}{a^2} + \frac{y^2}{b^2} + \frac{z^2}{c^2} = 1</m>.
        Geometrically, this because more difficult.
        However, using Lagrange Multipliers,
        we only need to change the constraint from the equation of the sphere to the equation of the ellipse.
        <men>
          \begin{array}{*4{>{\displaystyle}l}} V(x,y,z) = 8xyz \amp  \amp \hspace{1cm} g(x,y,z) = \frac{x^2}{a^2} + \frac{y^2}{b^2} + \frac{z^2}{c^2} = r^2 \amp  \\[1em] \nabla V = (8yx,8xz,8xy) \amp  \amp \hspace{1cm} \nabla g = \left( \frac{2x}{a^2}, \frac{2y}{b^2}, \frac{2z}{c^2} \right) \amp  \\[1em] \nabla V = \lambda \nabla g \amp  \amp  \amp  \\[1em] 8yz = \lambda \frac{2x}{a^2} \amp \hspace{1cm} 8xz = \lambda \frac{2y}{b^2} \amp \hspace{2cm} 8xy = \lambda \frac{2z}{c^2} \end{array}
        </men>
      </p>
      <p>
        We isolate for <m>x</m> in the first expression and substitute in the second.
        <md>
          <mrow>x \amp  = \frac{4z^2 yz}{\lambda} \hspace{2cm} 8 \left( \frac{4a^2yz}{\lambda} \right) z = \frac{\lambda 2y}{b^2}</mrow>
          <intertext>We solve for <m>z</m> (again, careful with <m>y=0</m>).</intertext>
          <mrow>16a^2 b^2 z^2 \amp  = \lambda^2 \implies 4abz = \lambda \implies z = \frac{\lambda}{4ab}</mrow>
          <intertext>We have symmetry again in the variables.</intertext>
          <mrow>x \amp  = \frac{\lambda}{4bc} \hspace{2cm} y = \frac{\lambda}{4ac}</mrow>
          <intertext>We substitute <m>x</m>, <m>y</m> and <m>z</m> in the constraint and solve for <m>\lambda</m>.</intertext>
          <mrow>\frac{x^2}{a^2} + \frac{y^2}{b^2} + \frac{z^2}{c^2} \amp  = 3 \left( \frac{\lambda^2}{16a^2b^2c^2} \right) = 1 \implies \lambda = \frac{4abc}{\sqrt{3}}</mrow>
          <intertext>We use the value of <m>\lambda</m> to determine the other variables.</intertext>
          <mrow>x \amp  = \frac{a}{\sqrt{3}} \hspace{2cm} y = \frac{b}{\sqrt{3}} \hspace{2cm} z = \frac{c}{\sqrt{3}}</mrow>
          <mrow>V \amp  = \frac{8abc}{3\sqrt{3}}</mrow>
        </md>
      </p>
      <p>
        The volume of the ellipsoid is <m>\frac{4}{3} \pi abc</m>,
        so as a fraction of that volume,
        this is <m>\frac{2}{\sqrt{3}\pi}</m> times the volume of the ellipse,
        a very believable fraction.
        Again, the <m>x=0</m>,
        <m>y=0</m> or <m>z=0</m> cases are discounted since they would lead to zero area and we are looking for a maximum.
      </p>
    </statement>
  </example>
  <example>
    <statement>
      <p>
        We can use Lagrange multipliers with several constraints for higher dimensional problems.
        Consider a plane <m>x +y+ z = 12</m> and a parabaloid <m>z = x^2 +y^2</m>.
        Their intersection is an ellipse in <m>\RR^3</m>.
        I'd like to find its highest point and its lowest point,
        thinking of <m>z</m> as elevation.
        In Lagrange Multipliers,
        rhe function <m>f(x,y,z) = z</m> is simply height,
        and the two equations are the constraints.
        <men>
          \begin{array}{*3{>{\displaystyle}l}} f(x,y,z) = z \amp \hspace{1cm} g(x,y,z) = x + y + z = 11 \amp \hspace{1cm} h(x,y,z) = x^2 + y^2 - z = 0 \\ \nabla f = (0,0,1) \amp \hspace{1cm} \nabla g = (1,1,1) \amp \hspace{1cm} \nabla h = (2x, 2y, -1) \\ \nabla f = \lambda \nabla g + \mu \nabla h \amp  \amp  \\ 0 = \lambda + 2 x \mu \amp \hspace{1cm} 0 = \lambda + 2y \mu \amp \hspace{1cm} 1 = \lambda - \mu \end{array}
        </men>
      </p>
      <p>
        This system is relatively straightforward, even with five variables.
        We can solve for <m>\lambda</m> in the first two equation and equate the results.
        <md>
          <mrow>2x\mu \amp  = \lambda = 2 y \mu \implies x = y \ \ \ ( \mu \neq 0)</mrow>
          <intertext>We put <m>x</m> and <m>y</m> into the <m>h</m> constraint.</intertext>
          <mrow>z \amp  = 2x^2</mrow>
          <intertext>Then we put this expressionv for <m>z</m>, and replace <m>y</m> with <m>x</m> in the <m>g</m> constraint. This result is an expression solely in <m>x</m>, so we can solve for values of <m>x</m>.</intertext>
          <mrow>2x + 2x^2 \amp  = 12 \implies x = -3 \text{ or }  x = 2</mrow>
          <intertext>We know the other variables in terms of <m>x</m>, so values of <m>x</m> determine values of <m>y</m> and <m>z</m>.</intertext>
          <mrow>x \amp  = -3 \implies y = -3 \ \ z = 18</mrow>
          <mrow>x \amp  = 2 \implies y = 2 \ \ z = 8</mrow>
        </md>
      </p>
      <p>
        We can simply look at the <m>z</m> value,
        since we are trying to maximize it.
        We see a maximum at <m>(-3, -3, 18)</m> and the minimum at <m>(2,2,8)</m>.
      </p>
    </statement>
  </example>
  <example>
    <statement>
      <p>
        As we've seen in these examples,
        constrained optimization is a particularly useful tool for sovling complicated geometry problems.
        Here is another such problem.
        Say we have the equation of a very general ellipse centred at the origin,
        such as <m>17x^2 + 12xy + 8y^2 = 100</m>.
        Since this ellipse has an <m>xy</m> term,
        it is not oriented along any axis <mdash/> it's on some slanted plane through the origin.
        So we don't know, from inspection,
        what is major and minor semi-axes are.
        However, we can ask for the points further from and closest too the origin.
        That's asking for the min and max of the funciton
        <m>f(x,y) = x^2 + y^2</m> on the constraint which is the equation of the ellipse.
        <men>
          \begin{array}{*2{>{\displaystyle}l}} f(x,y) = x^2 + y^2 \amp \hspace{2cm} g(x,y) = 17x^2 + 12xy + 8y^2 = 100 \\ \nabla f = (2x, 2y) \amp \hspace{2cm} \nabla g = (34x + 12y, 12x + 16y) \\ \nabla f = \lambda \nabla g \amp  \\ 2x = \lambda( 34x + 12y) \amp 2y = \lambda( 12x + 16y) \end{array}
        </men>
      </p>
      <p>
        We solve for <m>\lambda</m> in both equation and equate the results.
        <md>
          <mrow>\frac{-2x}{34x + 12 y} \amp  = \lambda = \frac{-2y}{12 x + 16 y}</mrow>
          <mrow>12x^2 + 16xy \amp  = 34 xy + 12y^2</mrow>
          <intertext>This is a bit tricky, since there are quadratic terms in both <m>x</m> and <m>y</m>. Turns out, though, we can get use out of isolating <m>y^2</m>.</intertext>
          <mrow>2x^2 - 3xy - 2y^2 \amp  = 0 \implies y^2 = x^2 - \frac{3}{2} xy</mrow>
          <intertext>We replace <m>y^2</m> in the constraint. We are fortunate, since this replacement cancelled off the <m>xy</m> term and leaves us just with an expression in <m>x</m>.</intertext>
          <mrow>12 x^2 + 12 xy + 8 \left( x ^2 - \frac{3}{2} xy \right) \amp  = 100</mrow>
          <mrow>12x^2 + 8x^2 \amp  = 100 \implies x = \pm 2</mrow>
          <mrow>x \amp  = 2 \implies 8 - 6y - 2y^2 = 0 \implies y = 1, -4</mrow>
          <mrow>x \amp  = -2 \implies 8 + 6y - 2y^2 = 0 \implies y = -1, 4</mrow>
        </md>
      </p>
      <p>
        This gives us the four points <m>(2,1)</m>, <m>(-2,-1)</m>,
        <m>(2,-4)</m> and <m>(-2,4)</m>.
        The semi-major axis is the distance to the further point,
        and the semi-minor axis is the distance to the closet point
        (from the origin).
        Therefore, the semi-major axis is
        <m>\sqrt{20}</m> units long along the line in the direction <m>(2,-4)</m> and the semi-minor axis is
        <m>\sqrt{5}</m> units long in the direction <m>(2,1)</m>.
      </p>
    </statement>
  </example>
</section>