<section xml:id="taylor-series-examples">
  <title>Examples</title>
  <p>
    Let's try to calculate some Taylor series for important functions.
  </p>
  <example>
    <statement>
      <p>
        We start with the most important function in calculus:
        <m>e^x</m>.
        The derivatives of <m>e^x</m> are just <m>e^x</m>.
        If we centre a series at <m>x=0</m>,
        then all these derivatives evaluate to <m>1</m>.
        Therefore
        <me>
          e^x = \sum_{n=0}^\infty \frac{1}{n!}x^n = 1 + x + \frac{x^2}{2} + \frac{x^3}{6} + \frac{x^4}{24} + \frac{x^5}{120} + \ldots
        </me>
      </p>
      <p>
        We can check that the radius of convergence for this series is <m>R = \infty</m>,
        so this is an expression for <m>e^x</m> which works for all real numbers.
      </p>
    </statement>
  </example>
  <p>
    As an aside,
    this finally allows for the proper definition of the exponential function.
    For <m>r = \frac{a}{b}</m> a rational number,
    <m>a^r = \sqrt[b]{x^a}</m>, which was well understood.
    But if <m>r</m> is irrational,
    we previously had no idea what <m>a^r</m> actually was nor how to calculate it.
    We worked on faith that the exponential function <m>e^x</m> was well defined for irrational numbers.
    Now, however, we can use this series.
    The value of <m>e^{\pi}</m>,
    which was completely opaque and mysterious before, is now given by a series.
    <me>
      e^{\pi} = \sum_{n=0}^\infty \frac{\pi^n}{n!} = 1 + \pi + \frac{\pi^2}{2} + \frac{\pi^3}{6} + \frac{\pi^4}{24} + \frac{\pi^5}{120} + \ldots
    </me>
  </p>
  <p>
    Other important properties of the exponential function can be calculated from the series.
    Let's differentiate the series.
    (We use a shift in the series in the last step.)
    <me>
      \frac{d}{dx} e^x = \frac{d}{dx} \sum_{n=0}^\infty \frac{1}{n!} x^n = \sum_{n=1}^\infty \frac{1}{n!} n x^{n-1} = \sum_{n=1}^\infty \frac{1}{(n-1)!} x^{n-1} = \sum_{n=0}^\infty \frac{1}{n!} x^n = e^x
    </me>
  </p>
  <p>
    This recovers the fact that the exponential function is its own derivative.
  </p>
  <example>
    <statement>
      <p>
        Let's integrate the geometric series
        (we set the integration constant to zero).
        <md>
          <mrow>\int \sum_{n=0}^\infty x^n dx \amp  = \int \frac{1}{1-x} dx</mrow>
          <mrow>\sum_{n=0}^\infty \frac{x^{n+1}}{n+1} + C \amp  = -\ln |1-x| + C</mrow>
          <mrow>\sum_{n=0}^\infty \frac{x^{n+1}}{n+1} \amp  = -\ln (1-x)</mrow>
        </md>
      </p>
      <p>
        This gives a Tayor series for
        <m>- \ln (1-x)</m> centered at <m>\alpha = 0</m>.
        Integration can be a convenient way to calculate a series,
        since we didn't have to calculate all the coefficients directly.
      </p>
    </statement>
  </example>
  <example>
    <statement>
      <p>
        We remarked in the previous section that integration was easy for series.
        Let's look at the function <m>e^{x^2}</m>.
        It has no elementary anti-derivative,
        so we unable to integrate it with conventional methods.
        However, if we put <m>x^2</m> into the series for the exponential function,
        we get a series for <m>e^{x^2}</m>.
        <me>
          e^{x^2} = \sum_{n=0}^\infty \frac{x^{2n}}{n!}
        </me>
      </p>
      <p>
        Since this is a series, we can integrate it.
        <me>
          \int e^{x^2} dx = \sum_{n=0}^\infty \frac{x^{2n+1}}{(2n+1)n!} + C
        </me>
      </p>
      <p>
        This new series is the anti-derivative of <m>e^{x^2}</m>.
        We knew such a function should exist,
        and now we have a representation of it as a Taylor series. (The series has infinite radius of convergence).
      </p>
    </statement>
  </example>
  <example>
    <statement>
      <p>
        The Taylor series for sine and cosine are important examples.
        Centered at <m>x=0</m>, the derivatives of <m>\sin x</m> form a cycle:
        <m>\sin x</m>, <m>\cos x</m>,
        <m>-\sin x</m>, and <m>-\cos x</m>.
        Evaluated at <m>x=0</m>,
        these gives values of <m>0</m>,
        <m>1</m>, <m>0</m>, and <m>-1</m>.
        Therefore, we get the following expressions for the coefficient of the Taylor series. (Note we need to group the coefficients into odds and evens,
        writing <m>n= 2k</m> for evens and <m>n = 2k+1</m> for odds).
        <men>
          \begin{array}{*4{>{\displaystyle}l}} c_0 \amp  = f(0) = 0 \amp \hspace{2cm} c_1 \amp  = f^\prime(0) = 1 \\[1em] c_2 \amp  = \frac{f^{\prime\prime}(0)}{2!} = 0 \amp \hspace{2cm} c_3 \amp  = \frac{f^{\prime\prime\prime}(0)}{3!} = \frac{-1}{3!} \\[1em] c_4 \amp  = \frac{f^{(4)}(0)}{4!} = 0 \amp \hspace{2cm} c_5 \amp  = \frac{f^{(5)}(0)}{5!} = \frac{1}{5!} \\[1em] c_6 \amp  = \frac{f^{(6)}(0)}{6!} = 0 \amp \hspace{2cm} c_7 \amp  = \frac{f^{(7)}(0)}{7!} = \frac{-1}{7!} \\[1em] c_8 \amp  = \frac{f^{(8)}(0)}{8!} = 0 \amp \hspace{2cm} c_9 \amp  = \frac{f^{(9)}(0)}{9!} = \frac{1}{9!} \\[1em] c_{2k} \amp  = 0 \amp \hspace{2cm} c_{2k+1} \amp  = \frac{(-1)^k}{(2k+1)!} \end{array}
        </men>
      </p>
      <p>
        Using these coefficients,
        the Taylor series for sine centered at <m>\alpha = 0</m> is this series:
        <me>
          \sin x = \sum_{n=0}^\infty \frac{(-1)^k}{(2k+1)!} x^{2k+1}
        </me>
      </p>
      <p>
        The radius of convergence of this series is <m>R = \infty</m>,
        so it expresses <m>\sin x</m> for all real numbers.
        We can use similar steps to find the Taylor the series for cosine.
        <me>
          \cos x = \sum_{n=0}^\infty \frac{(-1)^k}{(2k)!} x^{2k}
        </me>
      </p>
      <p>
        The radius of convergence of this series is also <m>R = \infty</m>.
      </p>
    </statement>
  </example>
  <example>
    <statement>
      <p>
        Consider <m>f(x) = \ln x</m> centered at <m>\alpha = 1</m>.
        <men>
          \begin{array}{*4{>{\displaystyle}l}} f^\prime(x) \amp  = \frac{1}{x} \amp \hspace{2cm} f^{\prime \prime}(x) \amp  = \frac{-1}{x^2} \\[1em] f^{\prime \prime \prime}(x) \amp  = \frac{2}{x^3} \amp \hspace{2cm} f^{(4)}(x) \amp  = \frac{-6}{x^4} \end{array}
        </men>
      </p>
      <p>
        We look for a general patterns.
        There are three pieces: an alternating sign,
        a factorial multiplication growing in the numerator,
        an a power growing in the denominator.
        Careful to match the indices correctly to the first few elements of the pattern.
        <me>
          f^{(n)}(x) = \frac{(-1)^{n-1}(n-1)!}{x^n} \hspace{2cm} f^{(n)}(1) = (-1)^{n-1}(n-1)!
        </me>
      </p>
      <p>
        Once we have the general pattern,
        we evaluate it at the centre point and then we put it into the Taylor series form.
        <me>
          \ln x = \sum_{n=1}^\infty \frac{(-1)^{n-1}(n-1)!}{n!} (x-1)^n = \sum_{n=1}^\infty \frac{(-1)^{n-1}}{n} (x-1)^n
        </me>
      </p>
      <p>
        The radius of convergence is 1, found by ratio test.
      </p>
    </statement>
  </example>
  <example>
    <statement>
      <p>
        Consider <m>f(x) = \frac{1}{x^2}</m> centered at <m>\alpha = 3</m>.
        <md>
          <mrow>f^\prime(x) \amp  = \frac{-2}{x^3} \hspace{1cm} f^{\prime \prime}(x) = \frac{6}{x^4} \hspace{1cm} f^{\prime \prime \prime}(x) = \frac{-24}{x^5}</mrow>
          <intertext>We look for a general pattern as before.</intertext>
          <mrow>f^{(n)}(x) \amp  = \frac{(-1)^{n}(n+1)!}{x^{n+2}}</mrow>
          <intertext>We evaluate at the centre point.</intertext>
          <mrow>f^{(n)}(3) \amp  = \frac{(-1)^{n}(n+1)!}{3^{n+2}}</mrow>
          <intertext>We put this into the general Taylor series form.</intertext>
          <mrow>\ln x \amp  = \sum_{n=1}^\infty \frac{(-1)^{n}(n+1)!}{3^{n+2} n!} (x-3)^n = \sum_{n=1}^\infty \frac{(-1)^n (n+1)}{3^{n+2}} (x-3)^n</mrow>
        </md>
      </p>
      <p>
        The radius of convergence is 3, found by ratio test.
      </p>
    </statement>
  </example>
  <example>
    <statement>
      <p>
        Consider a function which has the following sequence of derivatives at <m>x=0</m>.
        <me>
          0, 1, 2, 0, -1, 4, 0, 1, 8, 0, -1, 16, 0, 1, 32, 0, -1, 64, \ldots
        </me>
      </p>
      <p>
        The pattern has a cycle of threes.
        All <m>3n</m> terms are 0.
        All <m>3n+1</m> terms are <m>(-1)^n</m>.
        All <m>3n+2</m> terms are <m>2^n</m>.
        Therefore, the series is best expressed in two pieces.
        <me>
          f(x) = \sum_{n=0}^\infty \frac{(-1)^n}{(3n+1)!} x^{3n+1} + \sum_{n=0}^\infty \frac{2^n}{(3n+2)!} x^{3n+2}
        </me>
      </p>
      <p>
        The radius of convergence is <m>\infty</m>, found by a ratio test.
      </p>
    </statement>
  </example>
</section>