<section xml:id="exponentials-and-trigonometry">
  <title>Exponentials and Trigonometry</title>
  <p>
    Taylor series allow us to investigate the strange relationship between exponentials and trigonometry.
    To understand this relationship,
    let's look at the series representation of the trigonometric functions.
  </p>
  <p>
    The Taylor series for sine and cosine were calculated in the previous setion.
    <me>
      \cos x = \sum_{n=0}^\infty \frac{(-1)^nx^{2n}}{(2n)!} \hspace{1cm} \sin x = \sum_{n=0}^\infty \frac{(-1)^nx^{2n+1}}{(2n+!)!}
    </me>
  </p>
  <p>
    The Taylor series for hyperbolic sine and hyperbolic cosine can be calculated similarly.
    <me>
      \cosh x = \sum_{n=0}^\infty \frac{x^{2n}}{(2n)!} \hspace{1cm} \sinh x = \sum_{n=0}^\infty \frac{x^{2n+1}}{(2n+!)!}
    </me>
  </p>
  <p>
    The similarities are uncanny:
    the only difference is the presence of the alternating <m>(-1)^n</m> term. (This is yet another reason that trigonometric and hyperbolic functions share similar names and identities).
    The exponential definition of the hyperbolics gives <m>e^x = \sinh x + \cosh x</m>.
    This identity is relatively easy to see in the series itself:
    if we combine the terms of the two hyperbolic series,
    we get all the terms of the exponential series.
  </p>
  <p>
    For the trigonometric functions,
    the connection is similar.
    However, it's not visible when we work solely with the real numbers.
    We need complex numbers to see the connection.
    Therefore, let <m>\imath^2 = -1</m>,
    or equivalently let <m>\pm \imath</m> be the roots of <m>x^2 + 1 = 0</m>.
    That is, <m>\imath</m> is a square root of <m>-1</m>.
    The number <m>\imath</m> is just a constant,
    so we can include it when we do series.
    The arithmetic changes a bit,
    but it behaves normally with multiplication and addition.
    We're going to calculate <m>e^{\imath x}</m> and see what happens.
    <md>
      <mrow>e^{\imath x} \amp  = \sum_{n=0}^\infty \frac{(\imath x)^n}{n!} = \sum_{n=0}^\infty \frac{\imath^n x^n}{n!}</mrow>
      <intertext>We split this series up into two series, one with the odd terms and one with the even terms.</intertext>
      <mrow>\amp  = \sum_{n=0}^\infty \frac{\imath^{2n} x^{2n}}{(2n)!} + \sum_{n=0}^\infty \frac{\imath^{2n+1} x^{2n+1}}{(2n+1)!}</mrow>
      <intertext>Now, anywhere we see <m>i^2</m>, we can replace it with <m>-1</m>.</intertext>
      <mrow>\amp  = \sum_{n=0}^\infty \frac{(-1)^n x^{2n}}{(2n)!} + \sum_{n=0}^\infty \frac{\imath (-1)^n x^{2n+1}}{(2n+1)!}</mrow>
      <intertext>Finally, pulling out <m>i</m> in the second terms, we find some familiar Taylor series.</intertext>
      <mrow>\amp  = \sum_{n=0}^\infty \frac{(-1)^n x^{2n}}{(2n)!} + \imath \sum_{n=0}^\infty \frac{(-1)^n x^{2n+1}}{(2n+1)!}</mrow>
      <mrow>e^{\imath x} \amp  = \cos x + \imath \sin x</mrow>
    </md>
  </p>
  <p>
    This result is called Euler's formula.
    It is very similar to the hyperbolic identity noted previously,
    <m>e^x = \cosh x + \sinh x</m>,
    but we need complex numbers to find it.
    We can rearrange this to get the opposite direction,
    giving exponential definitions for trigonometry to mirror hyperbolics:
    <me>
      \sin x = \frac{e^{\imath x} - e^{-\imath x}}{2\imath} \hspace{2cm} \cos x = \frac{e^{\imath x} + e^{-\imath x}}{2}
    </me>
  </p>
  <p>
    There is one very notable case of Euler's formula: let <m>x = \pi</m>.
    <me>
      e^{\imath \pi} = \cos \pi + \imath \sin \pi = 1
    </me>
  </p>
  <p>
    Alternatively,
    we can evaluate the trigonometric terms for someting very lovely.
    <me>
      e^{\imath \pi} + 1 = 0
    </me>
  </p>
  <p>
    This equation is perhaps the cleanest,
    most elegant relationship in mathematics.
    It relates, with no other terms,
    the five most important numbers:
    <m>0</m>, <m>1</m>, <m>\pi</m>,
    <m>e</m> and <m>\imath</m>.
  </p>
</section>